Reorganized ptypesTheory into 3 different theories
Split the definitions off from the theorems, and moved the reachability
stuff into its own theory.

hol/ptypesScript.sml
@@ -1,144 +1,7 @@
-open HolKernel bossLib boolLib boolSimps SatisfySimps Parse pairTheory optionTheory stringTheory finite_mapTheory sumTheory state_transformerTheory option_transformerTheory monadsyntax combinTheory lcsymtacs relationTheory pred_setTheory
+open HolKernel bossLib boolLib SatisfySimps Parse ptypes_definitionsTheory pred_setTheory finite_mapTheory optionTheory option_transformerTheory state_transformerTheory pairTheory combinTheory relationTheory lcsymtacs
 
 val _ = new_theory "ptypes"
 
-val _ = overload_on("=+", ``λk v f. f |+ (k,v)``);
-val _ = overload_on("=+", ``UPDATE``);
-val _ = overload_on("|+", ``λf kv. f |+ kv``);
-
-val _ = Hol_datatype `ptr = addr of 'a itself => num`;
-val num_to_ptr_def = Define `num_to_ptr n = addr (:'a) n`;
-val ptr_to_num_def = Define `ptr_to_num (addr _ n) = n`;
-val _ = export_rewrites ["num_to_ptr_def","ptr_to_num_def"];
-val _ = overload_on("pnil",``addr (:'a) 0``);
-
-val _ = type_abbrev ("varname",``:string``);
-val _ = type_abbrev ("funname",``:string``);
-val _ = Hol_datatype `AuxList = <| head : 'a ptr ; tail : AuxList ptr |>`;
-val _ = Hol_datatype `List = <| first : 'a AuxList ptr ; last : 'a AuxList ptr |>` ;
-
-val _ = Hol_datatype`
-  SetOfVariables = <| counter : num ; varnumb : num ; vars : Variable List ptr |> ;
-  Multiequation = <| erased : bool ; S : SetOfVariables ptr ; M : (VarTerm + FunTerm) List ptr |> ;
-  Variable = <| name : varname ; m : Multiequation ptr |> ;
-  FunTerm = <| fsymb : funname ; args : (VarTerm + FunTerm) List ptr |> ;
-  VarTerm = <| v : Variable ptr |>`;
-val _ = type_abbrev("Term", ``:(VarTerm + FunTerm)``);
-val _ = Hol_datatype `TempMultiequation = <| S : Term List ptr ; M : Term List ptr |>`;
-val _ = Hol_datatype `System = <| T : Multiequation List ptr ; U : Multiequation List ptr |>`;
-
-val _ = Hol_datatype `
-value = Variable_value of varname => num
-      | SetOfVariables_value of num => num => num
-      | Term_value of num + funname # num
-      | Multiequation_value of bool => num => num
-      | TempMultiequation_value of num => num
-      | System_value of num => num
-      | AuxList_value of num => num
-      | List_value of num => num`;
-
-val _ = type_abbrev("store", ``:num |-> value``);
-
-val _ = Hol_datatype `
-type = Variable_type
-     | SetOfVariables_type
-     | Term_type
-     | Multiequation_type
-     | TempMultiequation_type
-     | System_type
-     | AuxList_type of type
-     | List_type of type`;
-
-val _ = Hol_datatype `state = <| store : store ; cell_type : num -> type |>`;
-
-val (has_type_rules, has_type_ind, has_type_cases) = Hol_reln`
-  (typed_cell s c m ∧ (m ≠ 0 ⇒ (s.cell_type m = Multiequation_type)) ⇒
-   has_type s c (Variable_value _ m) Variable_type) ∧
-  (typed_cell s c m ∧ (m ≠ 0 ⇒ (s.cell_type m = List_type Variable_type)) ⇒
-   has_type s c (SetOfVariables_value _ _ m) SetOfVariables_type) ∧
-  (typed_cell s c m ∧ (m ≠ 0 ⇒ (s.cell_type m = Variable_type)) ⇒
-   has_type s c (Term_value (INL m)) Term_type) ∧
-  (typed_cell s c m ∧ (m ≠ 0 ⇒ (s.cell_type m = List_type Term_type)) ⇒
-   has_type s c (Term_value (INR (_,m))) Term_type) ∧
-  (typed_cell s c m1 ∧ (m1 ≠ 0 ⇒ (s.cell_type m1 = SetOfVariables_type)) ∧
-   typed_cell s c m2 ∧ (m2 ≠ 0 ⇒ (s.cell_type m2 = List_type Term_type)) ⇒
-   has_type s c (Multiequation_value _ m1 m2) Multiequation_type) ∧
-  (typed_cell s c m1 ∧ (m1 ≠ 0 ⇒ (s.cell_type m1 = List_type Term_type)) ∧
-   typed_cell s c m2 ∧ (m2 ≠ 0 ⇒ (s.cell_type m2 = List_type Term_type)) ⇒
-   has_type s c (TempMultiequation_value m1 m2) TempMultiequation_type) ∧
-  (typed_cell s c m1 ∧ (m1 ≠ 0 ⇒ (s.cell_type m1 = List_type Multiequation_type)) ∧
-   typed_cell s c m2 ∧ (m2 ≠ 0 ⇒ (s.cell_type m2 = List_type Multiequation_type)) ⇒
-   has_type s c (System_value m1 m2) System_type) ∧
-  (typed_cell s c m1 ∧ (m1 ≠ 0 ⇒ (s.cell_type m1 = AuxList_type type)) ∧
-   typed_cell s c m2 ∧ (m2 ≠ 0 ⇒ (s.cell_type m2 = AuxList_type type)) ⇒
-   has_type s c (List_value m1 m2) (List_type type)) ∧
-  (typed_cell s c m1 ∧ (m1 ≠ 0 ⇒ (s.cell_type m1 = type)) ∧
-   typed_cell s c m2 ∧ (m2 ≠ 0 ⇒ (s.cell_type m2 = AuxList_type type)) ⇒
-   has_type s c (AuxList_value m1 m2) (AuxList_type type)) ∧
-  (m ∈ c ∧ m ∈ FDOM s.store ⇒ typed_cell s c m) ∧
-  (0 ∉ FDOM s.store ⇒ typed_cell s c 0) ∧
-  ((FLOOKUP s.store n = SOME v) ∧ has_type s (n INSERT c) v (s.cell_type n) ⇒ typed_cell s c n)`;
-
-val typed_state_def = Define`
-   typed_state s = ∀n. n ∈ FDOM s.store ⇒ typed_cell s {} n`;
-
-val _ = type_abbrev("inject", ``:'a -> value``);
-val _ = type_abbrev("project", ``:value -> 'a option``);
-val _ = Hol_datatype`embed = <| type : type ; inject : 'a inject ; project : 'a project |>`;
-val inject_Variable_def = Define`
-  inject_Variable a = Variable_value a.name (ptr_to_num a.m)`;
-val project_Variable_def = Define`
-  (project_Variable (Variable_value name vars) = SOME (Variable name (num_to_ptr vars))) ∧
-  (project_Variable _ = NONE)`;
-val _ = overload_on("embed_Variable",``embed Variable_type inject_Variable project_Variable : Variable embed``);
-val inject_SetOfVariables_def = Define`
-  inject_SetOfVariables a = SetOfVariables_value a.counter a.varnumb (ptr_to_num a.vars)`;
-val project_SetOfVariables_def = Define`
-  (project_SetOfVariables (SetOfVariables_value counter varnumb vars) = SOME (SetOfVariables counter varnumb (num_to_ptr vars))) ∧
-  (project_SetOfVariables _ = NONE)`;
-val _ = overload_on("embed_SetOfVariables",``embed SetOfVariables_type inject_SetOfVariables project_SetOfVariables : SetOfVariables embed``);
-val inject_Term_def = Define`
-  (inject_Term (INL al) = Term_value (INL (ptr_to_num al.v))) ∧
-  (inject_Term (INR ar) = Term_value (INR (ar.fsymb, (ptr_to_num ar.args))))`;
-val project_Term_def = Define`
-  (project_Term (Term_value (INL v)) = SOME (INL (VarTerm (num_to_ptr v)))) ∧
-  (project_Term (Term_value (INR (fsymb, args))) = SOME (INR (FunTerm fsymb (num_to_ptr args)))) ∧
-  (project_Term _ = NONE)`;
-val _ = overload_on("embed_Term",``embed Term_type inject_Term project_Term : Term embed``);
-val inject_Multiequation_def = Define`
-  inject_Multiequation a = Multiequation_value a.erased (ptr_to_num a.S) (ptr_to_num a.M)`;
-val project_Multiequation_def = Define`
-  (project_Multiequation (Multiequation_value erased S_ M) = SOME (Multiequation erased (num_to_ptr S_) (num_to_ptr M))) ∧
-  (project_Multiequation _ = NONE)`;
-val _ = overload_on("embed_Multiequation",``embed Multiequation_type inject_Multiequation project_Multiequation : Multiequation embed``);
-val inject_TempMultiequation_def = Define`
-  inject_TempMultiequation a = TempMultiequation_value (ptr_to_num a.S) (ptr_to_num a.M)`;
-val project_TempMultiequation_def = Define`
-  (project_TempMultiequation (TempMultiequation_value S_ M) = SOME (TempMultiequation (num_to_ptr S_) (num_to_ptr M))) ∧
-  (project_TempMultiequation _ = NONE)`;
-val _ = overload_on("embed_TempMultiequation",``embed TempMultiequation_type inject_TempMultiequation project_TempMultiequation : TempMultiequation embed``);
-val inject_System_def = Define`
-  inject_System a = System_value (ptr_to_num a.T) (ptr_to_num a.U)`;
-val project_System_def = Define`
-  (project_System (System_value T_ U) = SOME (System (num_to_ptr T_) (num_to_ptr U))) ∧
-  (project_System _ = NONE)`;
-val _ = overload_on("embed_System",``embed System_type inject_System project_System : System embed``);
-val inject_AuxList_def = Define`
-  inject_AuxList a = AuxList_value (ptr_to_num a.head) (ptr_to_num a.tail)`;
-val project_AuxList_def = Define`
-  (project_AuxList (AuxList_value head tail) = SOME (AuxList (num_to_ptr head) (num_to_ptr tail))) ∧
-  (project_AuxList _ = NONE)`;
-val _ = overload_on("embed_AuxList", ``λemb:'a embed. embed (AuxList_type emb.type) inject_AuxList project_AuxList : 'a AuxList embed``);
-val inject_List_def = Define`
-  inject_List a = List_value (ptr_to_num a.first) (ptr_to_num a.last)`;
-val project_List_def = Define`
-  (project_List (List_value first last) = SOME (List (num_to_ptr first) (num_to_ptr last))) ∧
-  (project_List _ = NONE)`;
-val _ = overload_on("embed_List", ``λemb:'a embed. embed (List_type emb.type) inject_List project_List : 'a List embed``);
-val _ = export_rewrites["inject_Variable_def","project_Variable_def","inject_SetOfVariables_def","project_SetOfVariables_def","inject_Term_def","project_Term_def","inject_Multiequation_def","project_Multiequation_def","inject_TempMultiequation_def","project_TempMultiequation_def","inject_System_def","project_System_def","inject_AuxList_def","project_AuxList_def","inject_List_def","project_List_def"];
-
-val is_embed_def = Define`
-  is_embed emb = ∀a v. (emb.inject a = v) ⇔ (emb.project v = SOME a)`;
 local
   fun Cases_on_if p (g as (asl,tm)) = let
     val tm = find_term p tm handle HOL_ERR _ =>
@@ -161,157 +24,6 @@ in
   val is_embed_AuxList = Q.store_thm("is_embed_AuxList", `is_embed (embed_AuxList emb)`, tac);
   val is_embed_List = Q.store_thm("is_embed_List", `is_embed (embed_List emb)`, tac);
 end
-
-val raw_lookup_def = Define`
-  raw_lookup (emb:'a embed) (addr _ n : 'a ptr) =
-  do v <- (λs. (FLOOKUP s.store n, s)) ;
-     t <- (λs. (SOME (s.cell_type n), s)) ;
-     if t = emb.type then return (emb.project v) else OPTIONT_FAIL
-  od`;
-val _ = overload_on("lookup", ``λp:Variable ptr. raw_lookup embed_Variable p``);
-val _ = overload_on("lookup", ``λp:SetOfVariables ptr. raw_lookup embed_SetOfVariables p``);
-val _ = overload_on("lookup", ``λp:Term ptr. raw_lookup embed_Term p``);
-val _ = overload_on("lookup", ``λp:Multiequation ptr. raw_lookup embed_Multiequation p``);
-val _ = overload_on("lookup", ``λp:TempMultiequation ptr. raw_lookup embed_TempMultiequation p``);
-val _ = overload_on("lookup", ``λp:System ptr. raw_lookup embed_System p``);
-val _ = overload_on("lookup", ``λemb. raw_lookup (embed_AuxList emb)``);
-val _ = overload_on("lookup", ``λemb. raw_lookup (embed_List emb)``);
-
-val raw_assign_def = Define`
-  raw_assign (emb:'a embed) (addr _ n : 'a ptr) v =
-  λs. ((), s with <| store updated_by (n =+ (emb.inject v)) ;
-                     cell_type updated_by (n =+ emb.type) |>)`;
-val _ = overload_on("assign", ``λp:Variable ptr. raw_assign embed_Variable p``);
-val _ = overload_on("assign", ``λp:SetOfVariables ptr. raw_assign embed_SetOfVariables p``);
-val _ = overload_on("assign", ``λp:Term ptr. raw_assign embed_Term p``);
-val _ = overload_on("assign", ``λp:Multiequation ptr. raw_assign embed_Multiequation p``);
-val _ = overload_on("assign", ``λp:TempMultiequation ptr. raw_assign embed_TempMultiequation p``);
-val _ = overload_on("assign", ``λp:System ptr. raw_assign embed_System p``);
-val _ = overload_on("assign", ``λemb. raw_assign (embed_AuxList emb)``);
-val _ = overload_on("assign", ``λemb. raw_assign (embed_List emb)``);
-
-val dispose_def = Define`
-  dispose (addr _ n) = λs. ((), s with store updated_by (λs. s \\ n))`;
-
-val free_addr_def = Define`
-  free_addr = λs. (addr (:'a) (@n. n ≠ 0 ∧ n ∉ FDOM s.store), s)`;
-
-val raw_new_def = Define`raw_new emb v = do ptr <- free_addr ; raw_assign emb ptr v ; return ptr od`;
-val _ = overload_on("new", ``λv:Variable. raw_new embed_Variable v``);
-val _ = overload_on("new", ``λv:SetOfVariables. raw_new embed_SetOfVariables v``);
-val _ = overload_on("new", ``λv:Term. raw_new embed_Term v``);
-val _ = overload_on("new", ``λv:Multiequation. raw_new embed_Multiequation v``);
-val _ = overload_on("new", ``λv:TempMultiequation. raw_new embed_TempMultiequation v``);
-val _ = overload_on("new", ``λv:System. raw_new embed_System v``);
-val _ = overload_on("new", ``λemb. raw_new (embed_AuxList emb)``);
-val _ = overload_on("new", ``λemb. raw_new (embed_List emb)``);
-
-val _ = export_rewrites["raw_lookup_def","raw_assign_def","dispose_def","raw_new_def"];
-
-val CreateList_def = Define`
-  CreateList emb =
-  do l <- new emb (AuxList pnil pnil) ;
-     s <- new emb (List l l) ;
-     return s
-  od`;
-val _ = overload_on("CreateListOfTerms", ``CreateList embed_Term``);
-val _ = overload_on("CreateListOfMulteq", ``CreateList embed_Multiequation``);
-val _ = overload_on("CreateListOfTempMulteq", ``CreateList embed_TempMultiequation``);
-val _ = overload_on("CreateListOfVariables", ``CreateList embed_Variable``);
-
-val HeadOfList_def = Define`
-  HeadOfList emb s =
-  do s' <- lookup emb s ;
-     s'first' <- lookup emb s'.first ;
-     return s'first'.head
-  od`;
-val _ = overload_on("HeadOfListOfTerms", ``HeadOfList embed_Term``);
-val _ = overload_on("HeadOfListOfMulteq", ``HeadOfList embed_Multiequation``);
-val _ = overload_on("HeadOfListOfTempMulteq", ``HeadOfList embed_TempMultiequation``);
-val _ = overload_on("HeadOfListOfVariables", ``HeadOfList embed_Variable``);
-
-val EmptyList_def = Define`
-  EmptyList emb s =
-  do s' <- lookup emb s ;
-     return (s'.first = s'.last)
-  od`;
-val _ = overload_on("EmptyListOfTerms", ``EmptyList embed_Term``);
-val _ = overload_on("EmptyListOfMulteq", ``EmptyList embed_Multiequation``);
-val _ = overload_on("EmptyListOfTempMulteq", ``EmptyList embed_TempMultiequation``);
-val _ = overload_on("EmptyListOfVariables", ``EmptyList embed_Variable``);
-
-val TailOfList_def = Define`
-  TailOfList emb s =
-  do s' <- lookup emb s ;
-     l <- return s'.first ;
-     l' <- lookup emb l;
-     assign emb s (List l'.tail s'.last) ;
-     dispose l ;
-     return s
-  od`;
-val _ = overload_on("TailOfListOfTerms", ``TailOfList embed_Term``);
-val _ = overload_on("TailOfListOfMulteq", ``TailOfList embed_Multiequation``);
-val _ = overload_on("TailOfListOfTempMulteq", ``TailOfList embed_TempMultiequation``);
-val _ = overload_on("TailOfListOfVariables", ``TailOfList embed_Variable``);
-
-val AddToEndOfList_def = Define`
-  AddToEndOfList emb t s =
-  do l <- new emb (AuxList pnil pnil) ;
-     s' <- lookup emb s ;
-     assign emb s'.last (AuxList t l) ;
-     assign emb s (List s'.first l) ;
-     return s
-  od`;
-val _ = overload_on("AddToEndOfListOfTerms", ``AddToEndOfList embed_Term``);
-val _ = overload_on("AddToEndOfListOfMulteq", ``AddToEndOfList embed_Multiequation``);
-val _ = overload_on("AddToEndOfListOfTempMulteq", ``AddToEndOfList embed_TempMultiequation``);
-val _ = overload_on("AddToEndOfListOfVariables", ``AddToEndOfList embed_Variable``);
-
-val AddToFrontOfList_def = Define`
-  AddToFrontOfList emb t s =
-  do s' <- lookup emb s ;
-     l <- new emb (AuxList t s'.first) ;
-     assign emb s (List l s'.last) ;
-     return s
-  od`;
-val _ = overload_on("AddToFrontOfListOfTerms", ``AddToFrontOfList embed_Term``);
-val _ = overload_on("AddToFrontOfListOfMulteq", ``AddToFrontOfList embed_Multiequation``);
-val _ = overload_on("AddToFrontOfListOfTempMulteq", ``AddToFrontOfList embed_TempMultiequation``);
-val _ = overload_on("AddToFrontOfListOfVariables", ``AddToFrontOfList embed_Variable``);
-
-val AppendLists_def = Define`
-  AppendLists emb t1 t2 =
-  do t2' <- lookup emb t2 ;
-     if t2'.first ≠ t2'.last then
-        do t1' <- lookup emb t1 ;
-           t2'first' <- lookup emb t2'.first ;
-           assign emb t1'.last (AuxList t2'first'.head t2'first'.tail) ;
-           assign emb t1 (List t1'.first t2'.last) ;
-           return ()
-        od
-     else return () ;
-     dispose t2'.first ;
-     dispose t2 ;
-     return t1
-  od`;
-val _ = overload_on("AppendListsOfTerms", ``AppendLists embed_Term``);
-val _ = overload_on("AppendListsOfMulteq", ``AppendLists embed_Multiequation``);
-val _ = overload_on("AppendListsOfTempMulteq", ``AppendLists embed_TempMultiequation``);
-val _ = overload_on("AppendListsOfVariables", ``AppendLists embed_Variable``);
-
-val (list_of_AuxList_rules, list_of_AuxList_ind, list_of_AuxList_cases) = Hol_reln`
-  (list_of_AuxList emb s last last []) ∧
-  (al ≠ last ∧
-   (FST ((do al' <- lookup emb al ;
-             (hd':'a) <- raw_lookup emb al'.head ;
-             return (hd',al'.tail)
-          od) s) =
-    SOME (hd',tl)) ∧
-   list_of_AuxList emb s last tl tl' ⇒
-   list_of_AuxList emb s last al (hd'::tl'))`;
-
-val list_of_List_def = Define`
-  list_of_List emb s l al' = ∃l'. (FST (lookup emb l s) = SOME l') ∧ list_of_AuxList emb s l'.last l'.first al'`;
 
 val NOTIN_INFINITE_FDOM_exists = Q.store_thm(
 "NOTIN_INFINITE_FDOM_exists",
@@ -464,7 +176,7 @@ val assign_comm = Q.store_thm(
  (SND (raw_assign emb1 p1 v1 (SND (raw_assign emb2 p2 v2 s))) =
   SND (raw_assign emb2 p2 v2 (SND (raw_assign emb1 p1 v1 s))))`,
 Cases_on `p1` >> Cases_on `p2` >> srw_tac [][] >>
-srw_tac [][theorem "state_component_equality",FUN_EQ_THM,APPLY_UPDATE_THM] >>
+srw_tac [][state_component_equality,FUN_EQ_THM,APPLY_UPDATE_THM] >>
 srw_tac [][GSYM fmap_EQ,INSERT_COMM] >>
 srw_tac [][FUN_EQ_THM,FAPPLY_FUPDATE_THM] >>
 srw_tac [][]);
@@ -487,95 +199,6 @@ val ptr_equality = Q.store_thm(
 `(ptr_to_num p1 = ptr_to_num p2) ⇔ (p1 = p2)`,
 Cases_on `p1` >> Cases_on `p2` >> srw_tac [][] >>
 PROVE_TAC [ITSELF_UNIQUE]);
-
-val (reach1_rules, reach1_ind, reach1_cases) = Hol_reln`
-  (reach1 m (Variable_value _ m)) ∧
-  (reach1 m (SetOfVariables_value _ _ m)) ∧
-  (reach1 m (Term_value (INL m))) ∧
-  (reach1 m (Term_value (INR (_,m)))) ∧
-  (reach1 m (Multiequation_value _ m _)) ∧
-  (reach1 m (Multiequation_value _ _ m)) ∧
-  (reach1 m (TempMultiequation_value m _)) ∧
-  (reach1 m (TempMultiequation_value _ m)) ∧
-  (reach1 m (System_value m _)) ∧
-  (reach1 m (System_value _ m)) ∧
-  (reach1 m (List_value m _)) ∧
-  (reach1 m (List_value _ m)) ∧
-  (reach1 m (AuxList_value m _)) ∧
-  (reach1 m (AuxList_value _ m))`;
-
-val cell_reach1_def = Define`
-  cell_reach1 (s:store) m n = ∃v. (FLOOKUP s n = SOME v) ∧ reach1 m v`;
-val _ = overload_on("cell_reach",``λs. RTC (cell_reach1 s)``);
-
-val reach_def = Define`
-  reach s m v = ∃n. reach1 n v ∧ cell_reach s m n`;
-
-val cell_reach_FUPDATE_end = Q.store_thm(
-"cell_reach_FUPDATE_end",
-`cell_reach (s |+ (m,w)) m n ⇔ cell_reach s m n`,
-reverse EQ_TAC >- (
-  map_every qid_spec_tac [`n`,`m`] >>
-  ho_match_mp_tac RTC_INDUCT_RIGHT1 >>
-  srw_tac [][cell_reach1_def] >>
-  qmatch_assum_rename_tac `FLOOKUP s p = SOME v` [] >>
-  Cases_on `m = p` >- PROVE_TAC [RTC_REFL] >>
-  `FLOOKUP (s |+ (m,w)) p = SOME v` by PROVE_TAC [FLOOKUP_UPDATE] >>
-  PROVE_TAC [cell_reach1_def,RTC_RULES_RIGHT1] ) >>
-qsuff_tac `!s0 s m n. cell_reach s m n ⇒ (s = s0 |+ (m,w)) ⇒ cell_reach s0 m n`
->- srw_tac [][] >>
-ntac 2 gen_tac >>
-ho_match_mp_tac RTC_INDUCT_RIGHT1 >>
-srw_tac [][cell_reach1_def] >>
-qmatch_assum_rename_tac `FLOOKUP (s0 |+ (m,w)) p = SOME v` [] >>
-Cases_on `m=p` >- PROVE_TAC [RTC_REFL] >>
-`FLOOKUP s0 p = SOME v` by PROVE_TAC [FLOOKUP_UPDATE] >>
-PROVE_TAC [cell_reach1_def,RTC_RULES_RIGHT1]);
-
-val reach_FUPDATE_end = Q.store_thm(
-"reach_FUPDATE_end",
-`reach (s |+ (m,w)) m v ⇔ reach s m v`,
-srw_tac [][reach_def,cell_reach_FUPDATE_end]);
-
-val cell_reach_bound = Q.store_thm(
-"cell_reach_bound",
-`cell_reach s m n ∧ n ≠ m ⇒ n ∈ FDOM s`,
-srw_tac [][Once RTC_CASES2,cell_reach1_def,FLOOKUP_DEF]);
-
-val FLOOKUP_reach_imp_cell_reach = Q.store_thm(
-"FLOOKUP_reach_imp_cell_reach",
-`(FLOOKUP s n = SOME v) ∧ reach s m v ⇒ cell_reach s m n`,
-srw_tac [][reach_def] >>
-srw_tac [SATISFY_ss][Once RTC_CASES2,cell_reach1_def]);
-
-val has_type_assign_unreachable = Q.store_thm(
-"has_type_assign_unreachable",
-`(∀c v t. has_type s c v t ⇒ ¬ reach s.store m v ⇒ has_type (s with store updated_by (m =+ w)) c v t) ∧
- (∀c n. typed_cell s c n ⇒ ¬ cell_reach s.store m n ⇒ typed_cell (s with store updated_by (m =+ w)) c n)`,
-ho_match_mp_tac has_type_ind >>
-reverse (srw_tac [][]) >- (
-  srw_tac [][Once has_type_cases,FLOOKUP_UPDATE] >>
-  PROVE_TAC [RTC_REFL,FLOOKUP_reach_imp_cell_reach] )
->- (
-  srw_tac [][Once has_type_cases] >>
-  PROVE_TAC [RTC_REFL] )
->- srw_tac [][Once has_type_cases] >>
-fsrw_tac [][reach_def,reach1_cases] >>
-srw_tac [][Once has_type_cases] >>
-first_x_assum match_mp_tac >>
-PROVE_TAC []);
-
-val has_type_remove_unreachable = Q.store_thm(
-"has_type_remove_unreachable",
-`(∀c v t. has_type s c v t ⇒ ¬ reach s.store m v ⇒ has_type (s with store updated_by combin$C $\\ m) c v t) ∧
- (∀c n. typed_cell s c n ⇒ ¬ cell_reach s.store m n ⇒ typed_cell (s with store updated_by combin$C $\\ m) c n)`,
-ho_match_mp_tac has_type_ind >>
-reverse (srw_tac [][]) >- (
-  srw_tac [][Once has_type_cases,DOMSUB_FLOOKUP_THM] >>
-  PROVE_TAC [RTC_REFL,FLOOKUP_reach_imp_cell_reach] ) >>
-srw_tac [][Once has_type_cases] >>
-fsrw_tac [][reach_def,reach1_cases] >>
-PROVE_TAC [RTC_RULES]);
 
 val typed_cell_def = Q.store_thm(
 "typed_cell_def",
@@ -604,7 +227,7 @@ val has_type_assign_unbound = Q.store_thm(
           has_type (s with <|store updated_by (m =+ w); cell_type updated_by (m =+ a)|>) c v t) ∧
  (∀c n. typed_cell s c n ⇒ m ≠ 0 ∧ m ∉ FDOM s.store ∧ m ∉ c ⇒
         typed_cell (s with <|store updated_by (m =+ w); cell_type updated_by (m =+ a)|>) c n)`,
-ho_match_mp_tac (theorem "has_type_strongind") >>
+ho_match_mp_tac has_type_strongind >>
 reverse (srw_tac [][]) >- (
   fsrw_tac [][] >>
   srw_tac [][Once has_type_cases,FLOOKUP_UPDATE,APPLY_UPDATE_THM] >>
@@ -635,7 +258,7 @@ val has_type_assign_cached_unbound = Q.store_thm(
           has_type (s with <|store updated_by (m =+ w); cell_type updated_by (m =+ a)|>) c v t) ∧
  (∀c n. typed_cell s c n ⇒ m ∈ c ∧ m ∉ FDOM s.store ⇒
         typed_cell (s with <|store updated_by (m =+ w); cell_type updated_by (m =+ a)|>) c n)`,
-ho_match_mp_tac (theorem "has_type_strongind") >>
+ho_match_mp_tac has_type_strongind >>
 reverse (srw_tac [][]) >- (
   fsrw_tac [][] >>
   srw_tac [][typed_cell_def,FLOOKUP_UPDATE,APPLY_UPDATE_THM] >>
@@ -670,9 +293,6 @@ val assign_FDOM = Q.store_thm(
 Cases_on `p` >> srw_tac [][]);
 val _ = export_rewrites["assign_FDOM"];
 
-val wfstate_def = Define`
-  wfstate s = typed_state s ∧ 0 ∉ FDOM s.store`;
-
 val free_addr_neq_0 = Q.store_thm(
 "free_addr_neq_0",
 `ptr_to_num (FST (free_addr s)) ≠ 0`,
@@ -700,26 +320,6 @@ srw_tac [][] >>
 (has_type_assign_unbound |> CONJUNCT2 |> MP_CANON |> match_mp_tac) >>
 srw_tac [][] >>
 fsrw_tac [][typed_state_def]);
-
-val cell_reach_typed_state_unbound_eq_0 = Q.store_thm(
-"cell_reach_typed_state_unbound_eq_0",
-`typed_state s ∧ cell_reach s.store m n ∧ m ≠ n ∧ m ∉ FDOM s.store ⇒ (m = 0)`,
-REWRITE_TAC [GSYM AND_IMP_INTRO] >>
-strip_tac >>
-map_every qid_spec_tac [`n`,`m`] >>
-ho_match_mp_tac RTC_INDUCT_RIGHT1 >>
-srw_tac [][] >>
-fsrw_tac [][cell_reach1_def] >>
-qmatch_assum_rename_tac `FLOOKUP s.store p = SOME v` [] >>
-`p ∈ FDOM s.store` by fsrw_tac [][FLOOKUP_DEF] >>
-Cases_on `m = n` >> srw_tac [][] >>
-imp_res_tac typed_state_def >>
-fsrw_tac [][Once has_type_cases] >>
-fsrw_tac [][] >> srw_tac [][] >>
-fsrw_tac [][reach1_cases] >> srw_tac [][] >>
-fsrw_tac [][Once has_type_cases] >>
-fsrw_tac [][Once has_type_cases] >>
-fsrw_tac [][FLOOKUP_DEF] );
 
 val AddToFrontOfList_wfstate = Q.store_thm(
 "AddToFrontOfList_wfstate",
@@ -772,7 +372,7 @@ Cases_on `p = n` >- (
     qsuff_tac `s with <|store updated_by x1; store updated_by x2; cell_type updated_by x4|> =
                s with <|store updated_by x1; cell_type updated_by x3; store updated_by x2; cell_type updated_by x4|>`
     >- srw_tac [][] >>
-    srw_tac [][theorem "state_component_equality",Abbr`x3`,Abbr`x4`,FUN_EQ_THM,APPLY_UPDATE_THM] >>
+    srw_tac [][state_component_equality,Abbr`x3`,Abbr`x4`,FUN_EQ_THM,APPLY_UPDATE_THM] >>
     srw_tac [][] ) >>
   map_every Q.UNABBREV_TAC [`x1`,`x2`,`x3`,`x4`,`c`,`v`,`t`] >>
   (has_type_assign_bound |> CONJUNCT1 |> MP_CANON |> match_mp_tac) >>
@@ -793,7 +393,7 @@ Cases_on `p = m` >- (
     qsuff_tac `s with <|store updated_by x1; store updated_by x2; cell_type updated_by x4|> =
                s with <|store updated_by x1; cell_type updated_by x3; store updated_by x2; cell_type updated_by x4|>`
     >- srw_tac [][] >>
-    srw_tac [][theorem "state_component_equality",Abbr`x3`,Abbr`x4`,FUN_EQ_THM,APPLY_UPDATE_THM] >>
+    srw_tac [][state_component_equality,Abbr`x3`,Abbr`x4`,FUN_EQ_THM,APPLY_UPDATE_THM] >>
     srw_tac [][] >> srw_tac [][] ) >>
   map_every Q.UNABBREV_TAC [`x1`,`x2`,`x3`,`x4`,`c`,`v`,`t`] >>
   (has_type_assign_bound |> CONJUNCT1 |> MP_CANON |> match_mp_tac) >>
@@ -819,7 +419,7 @@ qsuff_tac `typed_cell ((s with <|store updated_by x2; cell_type updated_by x4|>)
   qsuff_tac `s with <|store updated_by x1; store updated_by x2; cell_type updated_by x4|> =
              s with <|store updated_by x1; cell_type updated_by x3; store updated_by x2; cell_type updated_by x4|>`
   >- srw_tac [][] >>
-  srw_tac [][theorem "state_component_equality",Abbr`x3`,Abbr`x4`,FUN_EQ_THM,APPLY_UPDATE_THM] >>
+  srw_tac [][state_component_equality,Abbr`x3`,Abbr`x4`,FUN_EQ_THM,APPLY_UPDATE_THM] >>
   srw_tac [][] >> srw_tac [][] ) >>
 map_every Q.UNABBREV_TAC [`x1`,`x2`,`x3`,`x4`] >>
 (has_type_assign_bound |> CONJUNCT2 |> MP_CANON |> match_mp_tac) >>
