hol/reachScript.sml
@@ -1,0 +1,114 @@
+open HolKernel bossLib boolLib Parse SatisfySimps ptypes_definitionsTheory finite_mapTheory relationTheory lcsymtacs
+
+val _ = new_theory "reach"
+
+val (reach1_rules, reach1_ind, reach1_cases) = Hol_reln`
+  (reach1 m (Variable_value _ m)) ∧
+  (reach1 m (SetOfVariables_value _ _ m)) ∧
+  (reach1 m (Term_value (INL m))) ∧
+  (reach1 m (Term_value (INR (_,m)))) ∧
+  (reach1 m (Multiequation_value _ m _)) ∧
+  (reach1 m (Multiequation_value _ _ m)) ∧
+  (reach1 m (TempMultiequation_value m _)) ∧
+  (reach1 m (TempMultiequation_value _ m)) ∧
+  (reach1 m (System_value m _)) ∧
+  (reach1 m (System_value _ m)) ∧
+  (reach1 m (List_value m _)) ∧
+  (reach1 m (List_value _ m)) ∧
+  (reach1 m (AuxList_value m _)) ∧
+  (reach1 m (AuxList_value _ m))`;
+
+val cell_reach1_def = Define`
+  cell_reach1 (s:store) m n = ∃v. (FLOOKUP s n = SOME v) ∧ reach1 m v`;
+val _ = overload_on("cell_reach",``λs. RTC (cell_reach1 s)``);
+
+val reach_def = Define`
+  reach s m v = ∃n. reach1 n v ∧ cell_reach s m n`;
+
+val cell_reach_FUPDATE_end = Q.store_thm(
+"cell_reach_FUPDATE_end",
+`cell_reach (s |+ (m,w)) m n ⇔ cell_reach s m n`,
+reverse EQ_TAC >- (
+  map_every qid_spec_tac [`n`,`m`] >>
+  ho_match_mp_tac RTC_INDUCT_RIGHT1 >>
+  srw_tac [][cell_reach1_def] >>
+  qmatch_assum_rename_tac `FLOOKUP s p = SOME v` [] >>
+  Cases_on `m = p` >- PROVE_TAC [RTC_REFL] >>
+  `FLOOKUP (s |+ (m,w)) p = SOME v` by PROVE_TAC [FLOOKUP_UPDATE] >>
+  PROVE_TAC [cell_reach1_def,RTC_RULES_RIGHT1] ) >>
+qsuff_tac `!s0 s m n. cell_reach s m n ⇒ (s = s0 |+ (m,w)) ⇒ cell_reach s0 m n`
+>- srw_tac [][] >>
+ntac 2 gen_tac >>
+ho_match_mp_tac RTC_INDUCT_RIGHT1 >>
+srw_tac [][cell_reach1_def] >>
+qmatch_assum_rename_tac `FLOOKUP (s0 |+ (m,w)) p = SOME v` [] >>
+Cases_on `m=p` >- PROVE_TAC [RTC_REFL] >>
+`FLOOKUP s0 p = SOME v` by PROVE_TAC [FLOOKUP_UPDATE] >>
+PROVE_TAC [cell_reach1_def,RTC_RULES_RIGHT1]);
+
+val reach_FUPDATE_end = Q.store_thm(
+"reach_FUPDATE_end",
+`reach (s |+ (m,w)) m v ⇔ reach s m v`,
+srw_tac [][reach_def,cell_reach_FUPDATE_end]);
+
+val cell_reach_bound = Q.store_thm(
+"cell_reach_bound",
+`cell_reach s m n ∧ n ≠ m ⇒ n ∈ FDOM s`,
+srw_tac [][Once RTC_CASES2,cell_reach1_def,FLOOKUP_DEF]);
+
+val FLOOKUP_reach_imp_cell_reach = Q.store_thm(
+"FLOOKUP_reach_imp_cell_reach",
+`(FLOOKUP s n = SOME v) ∧ reach s m v ⇒ cell_reach s m n`,
+srw_tac [][reach_def] >>
+srw_tac [SATISFY_ss][Once RTC_CASES2,cell_reach1_def]);
+
+val has_type_assign_unreachable = Q.store_thm(
+"has_type_assign_unreachable",
+`(∀c v t. has_type s c v t ⇒ ¬ reach s.store m v ⇒ has_type (s with store updated_by (m =+ w)) c v t) ∧
+ (∀c n. typed_cell s c n ⇒ ¬ cell_reach s.store m n ⇒ typed_cell (s with store updated_by (m =+ w)) c n)`,
+ho_match_mp_tac has_type_ind >>
+reverse (srw_tac [][]) >- (
+  srw_tac [][Once has_type_cases,FLOOKUP_UPDATE] >>
+  PROVE_TAC [RTC_REFL,FLOOKUP_reach_imp_cell_reach] )
+>- (
+  srw_tac [][Once has_type_cases] >>
+  PROVE_TAC [RTC_REFL] )
+>- srw_tac [][Once has_type_cases] >>
+fsrw_tac [][reach_def,reach1_cases] >>
+srw_tac [][Once has_type_cases] >>
+first_x_assum match_mp_tac >>
+PROVE_TAC []);
+
+val has_type_remove_unreachable = Q.store_thm(
+"has_type_remove_unreachable",
+`(∀c v t. has_type s c v t ⇒ ¬ reach s.store m v ⇒ has_type (s with store updated_by combin$C $\\ m) c v t) ∧
+ (∀c n. typed_cell s c n ⇒ ¬ cell_reach s.store m n ⇒ typed_cell (s with store updated_by combin$C $\\ m) c n)`,
+ho_match_mp_tac has_type_ind >>
+reverse (srw_tac [][]) >- (
+  srw_tac [][Once has_type_cases,DOMSUB_FLOOKUP_THM] >>
+  PROVE_TAC [RTC_REFL,FLOOKUP_reach_imp_cell_reach] ) >>
+srw_tac [][Once has_type_cases] >>
+fsrw_tac [][reach_def,reach1_cases] >>
+PROVE_TAC [RTC_RULES]);
+
+val cell_reach_typed_state_unbound_eq_0 = Q.store_thm(
+"cell_reach_typed_state_unbound_eq_0",
+`typed_state s ∧ cell_reach s.store m n ∧ m ≠ n ∧ m ∉ FDOM s.store ⇒ (m = 0)`,
+REWRITE_TAC [GSYM AND_IMP_INTRO] >>
+strip_tac >>
+map_every qid_spec_tac [`n`,`m`] >>
+ho_match_mp_tac RTC_INDUCT_RIGHT1 >>
+srw_tac [][] >>
+fsrw_tac [][cell_reach1_def] >>
+qmatch_assum_rename_tac `FLOOKUP s.store p = SOME v` [] >>
+`p ∈ FDOM s.store` by fsrw_tac [][FLOOKUP_DEF] >>
+Cases_on `m = n` >> srw_tac [][] >>
+imp_res_tac typed_state_def >>
+fsrw_tac [][Once has_type_cases] >>
+fsrw_tac [][] >> srw_tac [][] >>
+fsrw_tac [][reach1_cases] >> srw_tac [][] >>
+fsrw_tac [][Once has_type_cases] >>
+fsrw_tac [][Once has_type_cases] >>
+fsrw_tac [][FLOOKUP_DEF] );
+
+val _ = export_theory ()
